Fixed Dafny solution and added lots of comments

dafny.dfy
@@ -1,81 +1,139 @@
-type pc_label = int
+// This is a specification of a simple concurrent algorithm from the paper
+// "Teaching Concurrency" by Leslie Lamport. In there are N processes and
+// two arrays of length N, x and y. Each process i executes the following
+// sequence of statements:
+//
+//     x[i] := 1;
+//     y[i] := x[(i-1) mod N];
+//
+// The reads and writes of each x[j] are assumed to be atomic. This
+// algorithm has the property that once all processes have finished, at
+// least one y[j] == 1.
+//
+// Dafny has no primitive notion of concurrency. One option is to use
+// the approach described in "Modeling Concurrency in Dafny" by Rustan
+// Leino [*], which is also how this algorithm would be modeled in TLA+.
+// However, I wanted to see if the algorithm could be modeled in a way
+// that preserves the simple sequential structure of each process. This
+// doesn't really matter for such a short and simple algorithm, but might
+// help when specifying algorithms in which processes have more control
+// states.
+//
+// The main challenge is specifying what it means for a process to yield
+// control to other processes after an atomic step. I believe that such a
+// specification is only meaningful in the context of a desired correctness
+// property and corresponding inductive invariant. We want it to be the case
+// that each atomic step of a process preserves the inductive invariant,
+// and from the perspective of a given process P, when P yields control, the
+// state of the system can be modified arbitrarily as long as:
+//     - the modification preserves the inductive invariant, and
+//     - the modification preserves the control state of P
+// I specified this with an unimplemented method Yield, which requires the
+// inductive invariant as a precondition (enforcing that every atomic step
+// preserves the inductive invariant), guarantees the inductive invariant
+// as a post condition, and guarantees that the yielding process's control
+// state doesn't change. This method, along with the algorithm and inductive
+// invariant, are captures in the class below.
+//
+// A downside of this approach is that there is no way to model
+// the scheduler in described in [*], so the methods Init and Proc
+// are never called. This means that the scheduler is implicit, and
+// there's no end to end verification argument.
+//
+// [*] http://leino.science/papers/krml260.pdf
 
-predicate Inv(pc: array<pc_label>, y: array<int>)
-requires pc.Length == y.Length;
-reads pc, y;
-{
-    (forall i : int :: 0 <= i < pc.Length ==> pc[i] == 2) ==>
-    exists i : int :: 0 <= i < y.Length && y[i] == 1
+// Possible control states of a process
+datatype pc_label = x_pc | y_pc | done
+
+class TeachingConcurrency {
+    var pc: array<pc_label>;
+    var x: array<int>;
+    var y: array<int>;
+
+    // The initial state of the system. This method doesn't actually
+    // do anything. It simply verifies that constraints on the initial
+    // state, as expressed by the requires clauses, imply the inductive
+    // invariant. I could have expressed the constraint on pc as a while
+    // loop or as a forall assignment statement. A while loop just seemed
+    // more complicated than necessary, and a forall assignment statement
+    // gave me some warning about triggers that I don't understand (because
+    // I've been too lazy to read about triggers).
+    method Init()
+    requires pc.Length == x.Length == y.Length;
+    requires forall i : int :: 0 <= i < pc.Length ==> pc[i] == x_pc;
+    requires x != y
+    requires 1 < pc.Length; // Non-empty set of processes.
+    ensures IndInv();
+    modifies pc;
+    {
+        // Need to convince Dafny of existence of a process
+        assert pc[1] != done;
+    }
+
+    // Specification of a process. This requires explicitly updating
+    // the control state (pc) of the process.
+    method Proc(i: int)
+    requires pc.Length == x.Length == y.Length;
+    requires 0 <= i < pc.Length;
+    requires IndInv();
+    ensures IndInv();
+    modifies x, y, pc;
+    {
+        x[i] := 1;
+        pc[i] := y_pc;
+        Yield(i);
+
+        y[i] := x[(i - 1) % x.Length];
+        pc[i] := done;
+        // The following assertions convince Dafny that IndInv
+        // holds. I couldn't figure out a simpler way to do so.
+        assert x_Inv();
+        assert AllDone() ==> x[(i - 1) % x.Length] == 1;
+        assert AllDone() ==> y[i] == 1;
+        Yield(i);
+    }
+
+    // All processes have finished.
+    predicate AllDone()
+    reads `pc, pc;
+    {
+        forall i : int :: 0 <= i < pc.Length ==> pc[i] == done
+    }
+
+    // The core correctness property of the algorithm. If every process
+    // has finished, then at least one y[i] == 1.
+    predicate Safety()
+    requires pc.Length == y.Length;
+    reads `pc, pc, `y, y;
+    {
+        AllDone() ==> exists i : int :: 0 <= i < y.Length && y[i] == 1
+    }
+
+    // Conjoining the following to Safety forms an inductive invariant.
+    // x_Inv just records that a x[i] = 1 once a process has moved                                                                                
+    // past x_pc.
+    predicate x_Inv()
+    requires pc.Length == x.Length;
+    reads `pc, pc, `x, x;
+    {
+        forall i : int ::
+            (0 <= i < pc.Length && pc[i] in {y_pc, done}) ==>
+            x[i] == 1
+    }
+
+    // The full inductive invariant.
+    predicate IndInv()
+    requires pc.Length == x.Length == y.Length;
+    reads `pc, pc, `x, x, `y, y;
+    {
+        Safety() && x_Inv() && x != y
+    }
+
+    method Yield(i: int)
+    requires pc.Length == x.Length == y.Length;
+    requires 0 <= i < pc.Length;
+    requires IndInv();
+    ensures IndInv();
+    ensures pc[i] == old(pc[i]);
+    modifies pc, x, y;
 }
-
-predicate x_Inv(pc: array<pc_label>, x: array<int>)
-requires pc.Length == x.Length;
-reads pc, x;
-{
-    forall i : int ::
-        (0 <= i < pc.Length && pc[i] in {1, 2}) ==>
-        x[i] == 1
-}
-
-predicate IndInv(pc: array<pc_label>, x: array<int>, y: array<int>)
-requires pc.Length == x.Length == y.Length;
-reads pc, x, y;
-{
-    Inv(pc, y) && x_Inv(pc, x)
-}
-
-method Yield(i: int, pc: array<pc_label>, x: array<int>, y: array<int>)
-requires pc.Length == x.Length == y.Length;
-requires 0 <= i < pc.Length;
-requires IndInv(pc, x, y);
-ensures IndInv(pc, x, y);
-ensures pc[i] == old(pc[i]) + 1;
-modifies pc, x, y;
-
-method Proc(i: int, pc: array<pc_label>, x: array<int>, y: array<int>)
-requires pc.Length == x.Length == y.Length;
-// requires pc != x; <- This doesn't seem to be necessary.
-requires pc != y;
-requires x != y;
-requires 0 <= i < pc.Length;
-requires pc[i] == 0;
-requires IndInv(pc, x, y);
-ensures IndInv(pc, x, y);
-modifies x, y, pc;
-{
-    x[i] := 1;
-    Yield(i, pc, x, y);
-    y[i] := x[(i - 1) % x.Length];
-    assert pc[i] == 1; // Why is this assertion necessary?
-    Yield(i, pc, x, y);
-}
-
-// IndInv didn't work first time
-// Did assertion based debugging. Started with
-// x_Inv and Inv immediately after x[i] := 1.
-// Neither held, Inv was missing yield requires !done[i]
-// (regular requires !done[i] had no effect).
-// x_Inv still didn't hold.
-
-// Problem with iterator stuff, asked on stack overflow, 
-// gave up on getting that to work, realized if I'm not going
-// to have main loop, no point in using iterators, might
-// as well just have a method per process, and a method yield
-// with IndInv as pre and post condition.
-
-// Property held vacuously at first, because I wrote
-// ensures pc[i] == old(pc)[i] + 1; instead of
-// ensures pc[i] == old(pc[i]) + 1; in Yield. I guess
-// the first one old(pc) is just a pointer to pc, which
-// hasn't changed. I figured this issue out with assertion
-// based debugging, eventually just putting an assert false in.
-// I was initially suspicious because I modified x_Inv to
-// something I believe to be insufficient (based on my
-// experience with the TLAPS proof). In particular, I reduced
-// the set of pc's under which x[i] == 1.
-
-// Needed to add that pc, x, y are not equal. Does this express
-// that the whole array is disjoint?
-
-// Annoyingly, I need to add assertion pc[i] == 1 after y update
-// (before y update doesn't help).
